Experiments with specializing O() specs with multiple parameters

examples/src/multivar_specialize.ml
@@ -4,3 +4,26 @@ let g (m, n) =
   done
 
 let f n = g (0, n)
+
+(*---------------*)
+
+let rec f2 m n =
+  if n > 0 then f2 (m+1) (n-1)
+  else if m > 0 then f2 (m-1) 0
+  else ()
+
+let f3 m n =
+  let nr = ref n in
+  let mr = ref m in
+  while !nr > 0 do
+    incr mr; decr nr
+  done;
+  while !mr > 0 do
+    decr mr
+  done
+
+let g2_1 n = f2 0 n
+let g2_2 m = f2 m 0
+
+let g3_1 n = f3 0 n
+let g3_2 m = f3 m 0
